Restore `balanceOf` spec and proof This file was accidentally overwritten while bringing in the changes from the `vc` generator in commit 6848b5.

Generated/erc20shim/ERC20Shim/fun_balanceOf_user.lean
@@ -1,9 +1,9 @@
 import Clear.ReasoningPrinciple
 
-import Generated.erc20shim.ERC20Shim.mapping_index_access_mapping_address_uint256_of_address
-
+-- import Generated.erc20shim.ERC20Shim.mapping_index_access_mapping_address_uint256_of_address
 import Generated.erc20shim.ERC20Shim.fun_balanceOf_gen
 
+import Generated.erc20shim.ERC20Shim.Predicate
 
 namespace Generated.erc20shim.ERC20Shim
 
@@ -11,13 +11,183 @@ section
 
 open Clear EVMState Ast Expr Stmt FunctionDefinition State Interpreter ExecLemmas OutOfFuelLemmas Abstraction YulNotation PrimOps ReasoningPrinciple Utilities Generated.erc20shim ERC20Shim
 
-def A_fun_balanceOf (var_ : Identifier) (var_account : Literal) (s₀ s₉ : State) : Prop := sorry
+section PleaseMoveTheseWhereAppropriatte
 
-lemma fun_balanceOf_abs_of_concrete {s₀ s₉ : State} {var_ var_account} :
-  Spec (fun_balanceOf_concrete_of_code.1 var_ var_account) s₀ s₉ →
-  Spec (A_fun_balanceOf var_ var_account) s₀ s₉ := by
+variable {jmp : Jump}
+
+@[simp]
+lemma hash_collision_evm_Checkpoint_eq_false : (Checkpoint jmp).evm.hash_collision = false := rfl
+
+end PleaseMoveTheseWhereAppropriatte
+
+def A_fun_balanceOf (var : Identifier) (var_account : Literal) (s₀ s₉ : State) : Prop :=
+  (∀ {erc20}, (IsERC20 erc20 s₀ ∧ s₀.evm.isEVMState) →
+  let account := Address.ofUInt256 var_account
+  IsERC20 erc20 s₉ ∧ preservesEvm s₀ s₉ ∧
+  s₉[var]!! = (erc20.balances.lookup account).getD 0 ∧
+  s₉.evm.hash_collision = false)
+  ∨ s₉.evm.hash_collision = true
+
+lemma fun_balanceOf_abs_of_concrete {s₀ s₉ : State} {var var_account} :
+  Spec (fun_balanceOf_concrete_of_code.1 var var_account) s₀ s₉ →
+  Spec (A_fun_balanceOf var var_account) s₀ s₉ := by
   unfold fun_balanceOf_concrete_of_code A_fun_balanceOf
-  sorry
+  rcases s₀ with ⟨evm, varstore⟩ | _ | _ <;> [simp only; aesop_spec; aesop_spec]
+  apply spec_eq
+  clr_funargs
+  rintro hasFuel ⟨s, mapping, code⟩
+  clr_varstore,
+
+  -- what we can get right now from mapping function
+  unfold A_mapping_index_access_mapping_address_uint256_of_address at mapping
+  clr_spec at mapping
+
+  -- Discharge the hash-colliding case immediately using `aesop_spec`.
+  rcases mapping with ⟨
+    ⟨preservesEvm, s_isOk, s_isEVMStatePreserved,
+    ⟨⟨keccak_value, keccak_using_keccak_value, hStore⟩,hHashCollision⟩⟩ | _, hHashCollision₁
+  ⟩ <;> [left; rcases s <;> aesop_spec]
+
+  intro erc20 is_erc20 s₀_isEVMState
+
+  obtain ⟨evmₛ, varstoreₛ, s_eq_ok⟩ := State_of_isOk s_isOk
+
+  have keccak : Finmap.lookup [↑↑(Address.ofUInt256 var_account), 0] s.evm.keccak_map = some (s["_2"]!!) := by
+    unfold store State.insert at hStore
+    unfold lookup!
+    aesop
+
+  rw [ ← Variables.balances_def
+    , s_eq_ok, get_evm_of_ok, ← s_eq_ok
+    ] at keccak
+
+  -- simplify contract
+  unfold reviveJump at code
+  simp [s_eq_ok] at code
+  rw [ ← State.insert_of_ok,  ← State.insert_of_ok, ← s_eq_ok ] at code
+  clr_varstore,
+
+  -- get underlying Preserved from preservesEvm
+  rw [ s_eq_ok, preservesEvm_of_insert, preservesEvm_of_insert ] at preservesEvm
+  have Preserved := Preserved_of_preservesEvm_of_Ok preservesEvm
+
+  refine' ⟨IsERC20_of_preservesEvm (by aesop) is_erc20, (by aesop), ?returns_correct_value⟩
+
+  rw [← code]
+  -- lookup balance
+  clr_varstore,
+  by_cases mem : Address.ofUInt256 var_account ∈ erc20.balances
+  · -- there is such account in balances
+    split_ands <;> [skip; aesop]
+
+    obtain ⟨address, has_address, balance⟩ := is_erc20.hasBalance mem
+
+    have address_def : s["_2"]!! = address := by
+      rw [s_eq_ok]
+      rw [← Option.some_inj]
+      trans
+      · exact Eq.symm (s_eq_ok ▸ keccak)
+      · exact (keccak_map_lookup_eq_of_Preserved_of_lookup Preserved has_address
+          ▸ has_address)
+
+    rw [address_def] at code ⊢
+    rw [ balance
+      , Option.getD_some
+      , State.get_evm_of_ok
+      , ← sload_eq_of_preserved Preserved
+      ]
+
+  · -- there is *no* such account in balances
+    -- so sload should return 0
+
+    split_ands <;> [skip; aesop]
+
+    rw [ Finmap.lookup_eq_none.mpr mem
+      , Option.getD_none
+      ]
+
+    -- in order to do that it should be given storage address outside of
+    -- it's domain
+    apply sload_of_not_mem_dom
+    have := State.get_evm_of_ok ▸ is_erc20.storageDom
+    rw [ ← storage_eq_of_preserved Preserved
+      , this
+      ]
+    clear this
+    simp only [ Finset.not_mem_union, Set.mem_toFinset, Set.mem_def, setOf, not_exists, not_and ]
+    have s_erc20 : IsERC20 erc20 (Ok evmₛ _) :=
+      IsERC20_of_ok_of_Preserved Preserved is_erc20
+
+    split_ands
+    -- address not in balances
+    · intro account account_mem_balances
+      obtain ⟨address, has_address, balance⟩ := is_erc20.hasBalance account_mem_balances
+      rw [ ← keccak
+        , keccak_map_lookup_eq_of_Preserved_of_lookup
+            Preserved has_address ]
+      by_contra h
+      have : [↑↑account, ERC20Private.balances] ∈ evmₛ.keccak_map.keys := by
+        rw [Finmap.mem_keys]
+        apply Finmap.lookup_isSome.mp
+        have := get_evm_of_ok ▸ has_address
+        rw [ ← keccak_map_lookup_eq_of_Preserved_of_lookup Preserved has_address
+          , this ]
+        simp
+      have IsEVMₛ : evmₛ.isEVMState := by aesop
+      have keccak_inj := IsEVMₛ.1 this (Eq.symm h)
+
+      rw [← Fin.ofNat''_eq_cast, ← Fin.ofNat''_eq_cast] at keccak_inj
+      unfold Fin.ofNat'' at keccak_inj
+      simp at keccak_inj
+      rw [Nat.mod_eq_of_lt, Nat.mod_eq_of_lt, Fin.val_eq_val] at keccak_inj
+      rw [keccak_inj] at account_mem_balances
+      exact (mem account_mem_balances)
+      · exact Address.ofUInt256_lt_UInt256_size
+      · exact Address.val_lt_UInt256_size
+
+    -- address not in allowances
+    · intro owner spender mem_allowances
+      obtain ⟨erc_address, erc_intermediate, owner_lookup, spender_lookup, eq⟩ :=
+        is_erc20.hasAllowance mem_allowances
+      rw [get_evm_of_ok] at owner_lookup spender_lookup
+      have spender_lookup_s := keccak_map_lookup_eq_of_Preserved_of_lookup Preserved spender_lookup
+      push_neg
+      use erc_intermediate
+      rw [ ← keccak ]
+      by_contra h
+      rw [not_and'] at h
+      apply h at owner_lookup
+      exact owner_lookup
+
+      rw [spender_lookup_s]
+      by_contra h
+      have : [↑↑spender, erc_intermediate] ∈ evmₛ.keccak_map.keys := by
+        rw [Finmap.mem_keys]
+        apply Finmap.lookup_isSome.mp
+        have := Eq.trans (Eq.symm spender_lookup_s) spender_lookup
+        rw [this]
+        simp
+      have IsEVMₛ : evmₛ.isEVMState := by aesop
+      have keccak_inj := IsEVMₛ.1 this h
+      simp at keccak_inj
+      have intermediate_ne_balances : erc_intermediate ≠ ERC20Private.balances := by
+        obtain blocked_range := get_evm_of_ok ▸ is_erc20.block_acc_range.2.1
+        rw [owner_lookup] at blocked_range
+        unfold not_mem_private at blocked_range
+        simp at blocked_range
+        rw [← Finset.forall_mem_not_eq] at blocked_range
+        have bal_mem_private: ERC20Private.balances ∈ ERC20Private.toFinset := by
+          unfold PrivateAddresses.toFinset
+          simp
+        specialize blocked_range ERC20Private.balances
+        exact blocked_range bal_mem_private
+
+      tauto
+    -- address not in reserved space
+    · -- NOTE: Technically can be a one liner with a bit more infrastructure for keccak.
+      -- QUESTION: I don't think it's worth revisiting post-haste; or is it?
+      have blocked_range := keccak ▸ get_evm_of_ok ▸ s_erc20.block_acc_range.1
+      exact not_mem_private_of_some blocked_range
 
 end
 
